proved decidability properties of basic definitions (sterms, cmds, sstates...), and extracted an OCaml TV with data types for LLVM ASTs and symbolic states.
An alternative is to define comparison functions on these terms, and
prove that these functions return true only when terms are indead equal.
That makes extracted code close to functions in Coq. The current
extraction was from decidability proofs, which are still readable, and
very close to what we will define them intuitively. These also give
equalities between terms (t1=t2 <-> sumbool (t1=t2) (~t1=t2)=left _) for free (trivially from decidability).



git-svn-id: https://webdav.seas.upenn.edu/svn/sol/vol@2552 eef5ea85-cc2e-0410-bd84-0fae1f012da8

src/TV/symexe_correct.v
@@ -19,6 +19,8 @@ Require Import symexe_sound.
 Require Import seop_llvmop.
 Require Import assoclist.
 Require Import ssa_props.
+Require Import symexe_dec.
+Require Import Coq.Bool.Sumbool.
 
 Export SimpleSE.
 
@@ -561,9 +563,56 @@ Qed.
 
 (* Correctness of the cmds validator *)
 
+
+Tactic Notation "bdestruct" ident(H) "as" ident(J1) ident(J2) :=
+     apply andb_true_iff in H; destruct H as [J1 J2].
+
+Tactic Notation "bdestruct3" ident(H) "as" ident(J1) ident(J2) ident(J3) :=
+     bdestruct H as H J3;
+     bdestruct H as J1 J2.
+
+Tactic Notation "bdestruct4" ident(H) "as" ident(J1) ident(J2) ident(J3) ident(J4) :=
+     bdestruct3 H as H J3 J4;
+     bdestruct H as J1 J2.
+
+Tactic Notation "bdestruct5" ident(H) "as" ident(J1) ident(J2) ident(J3) ident(J4) ident(J5) :=
+     bdestruct4 H as H J3 J4 J5;
+     bdestruct H as J1 J2.
+
+Ltac bdestructn H Js :=
+  match Js with
+  | nil => idtac
+  | ?J::nil => rename H into J
+  | ?J::?Js' => apply andb_true_iff in H; destruct H as [H J]; bdestructn H Js
+  end.
+
 Definition tv_cmds (nbs1 nbs2 : list nbranch) :=
-se_cmds sstate_init nbs1 =
-se_cmds sstate_init nbs2.
+sumbool2bool _ _ (sstate_dec (se_cmds sstate_init nbs1) (se_cmds sstate_init nbs2)).
+
+Ltac sumbool_simpl :=
+  repeat
+  match goal with
+  | [ H:sumbool2bool _ _ _ = true |- _ ] => apply sumbool2bool_true in H
+  | [ H:is_true(sumbool2bool _ _ _) |- _ ] => apply sumbool2bool_true in H
+  | [ H:tv_cmds _ _ = true |- _ ] => unfold is_true in H; apply sumbool2bool_true in H
+  | [ H:is_true(tv_cmds _ _) |- _ ] => unfold is_true in H; apply sumbool2bool_true in H
+  end.
+
+Ltac sumbool_subst :=
+  repeat
+  match goal with
+  | [ H:sumbool2bool _ _ _ = true |- _ ] => apply sumbool2bool_true in H; subst
+  | [ H:is_true(sumbool2bool _ _ _) |- _ ] => apply sumbool2bool_true in H; subst
+  end.
+
+Tactic Notation "sumbool_subst" "in" hyp(H) :=
+  apply sumbool2bool_true in H.
+
+Ltac bsplit :=
+  eapply andb_true_iff; split.
+
+Ltac repeat_bsplit :=
+  repeat (bsplit; auto using eq_sumbool2bool_true).
 
 Lemma tv_cmds__is__correct : forall TD nbs nbs' lc1 als1 gl Mem1 lc2 als2 Mem2 tr,
   uniq lc1 ->  
@@ -575,10 +624,10 @@ Lemma tv_cmds__is__correct : forall TD nbs nbs' lc1 als1 gl Mem1 lc2 als2 Mem2 t
     eqAL _ slc lc2.
 Proof.
   intros TD nbs nbs' lc1 als1 gl Mem1 lc2 als2 Mem2 tr Huniqc Wf Htv_cmds HdbCmds.
-  unfold tv_cmds in Htv_cmds.
   assert (Uniqs:=HdbCmds).
   apply se_dbCmds_preservation in Uniqs; auto.
   apply op_cmds__satisfy__se_cmds in HdbCmds; auto.
+  sumbool_simpl.
   rewrite Htv_cmds in HdbCmds.
   apply se_cmds__denote__op_cmds; auto.
 Qed.
@@ -590,21 +639,24 @@ match (sb1, sb2) with
   let st2 := se_cmds sstate_init nbs2 in
   let cl1 := se_call st1 call1 iscall1 in
   let cl2 := se_call st2 call2 iscall2 in
-  st1 = st2 /\ call1 = call2
+   (sumbool2bool _ _ (sstate_dec st1 st2)) &&
+   (sumbool2bool _ _ (cmd_dec call1 call2))
 end.
 
 Fixpoint tv_subblocks (sbs1 sbs2:list subblock) :=
 match (sbs1, sbs2) with
-| (nil, nil) => True
-| (sb1::sbs1', sb2::sbs2') => tv_subblock sb1 sb2 /\ tv_subblocks sbs1' sbs2' 
-| _ => False
+| (nil, nil) => true
+| (sb1::sbs1', sb2::sbs2') => 
+   (tv_subblock sb1 sb2) && (tv_subblocks sbs1' sbs2')
+| _ => false
 end.
 
 Fixpoint tv_phinodes (ps1 ps2:phinodes) :=
 match (ps1, ps2) with
-| (nil, nil) => True
-| (p1::ps1', p2::ps2') => p1=p2 /\ tv_phinodes ps1' ps2'
-| _ => False
+| (nil, nil) => true
+| (p1::ps1', p2::ps2') => 
+    sumbool2bool _ _ (phinode_dec p1 p2) && tv_phinodes ps1' ps2'
+| _ => false
 end.
 
 Definition tv_block (b1 b2:block) :=
@@ -612,50 +664,54 @@ match (b1, b2) with
 | (block_intro l1 ps1 cs1 tmn1, block_intro l2 ps2 cs2 tmn2) =>
   match (cmds2sbs cs1, cmds2sbs cs2) with
   | ((sbs1, nbs1), (sbs2, nbs2)) =>
-    l1 = l2 /\ 
-    tv_phinodes ps1 ps2 /\ 
-    tv_subblocks sbs1 sbs2 /\ 
-    tv_cmds nbs1 nbs2 /\ 
-    tmn1 = tmn2
+    sumbool2bool _ _ (eq_atom_dec l1 l2) &&
+    tv_phinodes ps1 ps2 &&
+    tv_subblocks sbs1 sbs2 &&
+    tv_cmds nbs1 nbs2 &&
+    sumbool2bool _ _ (terminator_dec tmn1 tmn2)
   end
 end.
 
 Fixpoint tv_blocks (bs1 bs2:blocks):=
 match (bs1, bs2) with
-| (nil, nil) => True
-| (b1::bs1', b2::bs2') => tv_block b1 b2 /\ tv_blocks bs1' bs2'
-| _ => False
+| (nil, nil) => true
+| (b1::bs1', b2::bs2') => tv_block b1 b2 && tv_blocks bs1' bs2'
+| _ => false
 end.
 
 Definition tv_fdef (f1 f2:fdef) :=
 match (f1, f2) with
 | (fdef_intro fh1 lb1, fdef_intro fh2 lb2) =>
-  fh1 = fh2 /\ tv_blocks lb1 lb2
+  sumbool2bool _ _ (fheader_dec fh1 fh2) &&
+  tv_blocks lb1 lb2
 end.
 
 Fixpoint tv_products (Ps1 Ps2:products):=
 match (Ps1, Ps2) with
-| (nil, nil) => True
+| (nil, nil) => true
 | (product_fdec f1::Ps1', product_fdec f2::Ps2') => 
-  f1 = f2 /\ tv_products Ps1' Ps2'
+  sumbool2bool _ _ (fdec_dec f1 f2) &&
+  tv_products Ps1' Ps2'
 | (product_fdef f1::Ps1', product_fdef f2::Ps2') => 
-  tv_fdef f1 f2 /\ tv_products Ps1' Ps2'
+  tv_fdef f1 f2 && tv_products Ps1' Ps2'
 | (product_gvar gvar1::Ps1', product_gvar gvar2::Ps2') => 
-  gvar1 = gvar2 /\ tv_products Ps1' Ps2'
-| _ => False
+  sumbool2bool _ _ (gvar_dec gvar1 gvar2) &&
+  tv_products Ps1' Ps2'
+| _ => false
 end.
 
 Definition tv_module (m1 m2:module) :=
 match (m1, m2) with
 | (module_intro TD1 Ps1, module_intro TD2 Ps2) =>
-  TD1 = TD2 /\ tv_products Ps1 Ps2
+  sumbool2bool _ _ (layouts_dec TD1 TD2) &&
+  tv_products Ps1 Ps2
 end.
 
 Fixpoint tv_system (S1 S2:system) :=
 match (S1, S2) with
-| (nil, nil) => True
-| (m1::S1', m2::S2') => tv_module m1 m2 /\ tv_system S1' S2'
-| _ => False
+| (nil, nil) => true
+| (m1::S1', m2::S2') => tv_module m1 m2 && tv_system S1' S2'
+| _ => false
 end.
 
 Lemma lookup_tv_blocks__tv_block : forall lb1 lb2 l0 B1,
@@ -675,7 +731,7 @@ Proof.
     destruct lb2.
       inversion H1.
 
-      destruct H1 as [J1 J2].
+      bdestruct H1 as J1 J2.
       assert (K:=H).
       apply uniqBlocks__uniqLabel2Block in H.
       apply mergeALs_inv in H2; auto.
@@ -693,7 +749,8 @@ Proof.
             unfold tv_block in J1.
             destruct (cmds2sbs c).
             destruct (cmds2sbs c0).
-            destruct J1 as [EQ _]; subst.
+            bdestruct5 J1 as J11 J12 J13 J14 J15.
+            sumbool_subst.
             destruct (l0==l2); inversion H2; subst; auto.
 
         simpl_env in K. apply uniqBlocks_inv in K. destruct K.
@@ -713,7 +770,7 @@ Lemma tv_blocks_nth_Some_inv : forall lb1 lb2 n B1,
   exists B2, 
     nth_error lb2 n = Some B2 /\ tv_block B1 B2.
 Proof.
-  intros.
+  intros lb1 lb2 n B1 H H0 H1 H2.
   assert (J:=H2).
   apply nth_error__lookupAL_genLabel2Block_blocks in H2; auto.
   destruct H2 as [l0 H2].
@@ -735,8 +792,9 @@ Lemma lookup_tv_fdef__tv_block : forall fh1 fh2 lb1 lb2 l0 B1,
     nth_error lb2 n = Some B2 /\
     lookupBlockViaLabelFromFdef (fdef_intro fh2 lb2) l0 = Some B2.
 Proof.
-  intros.
-  destruct H1 as [EQ Htv_blocks].
+  intros fh1 fh2 lb1 lb2 l0 B1 H H0 H1 H2.
+  bdestruct H1 as EQ Htv_blocks.
+  sumbool_subst.
   unfold lookupBlockViaLabelFromFdef in H2.
   unfold genLabel2Block_fdef in H2.
   eapply lookup_tv_blocks__tv_block; eauto.
@@ -748,13 +806,15 @@ Lemma tv_block__inv : forall B1 B2,
   tv_phinodes (getPhiNodesFromBlock B1) (getPhiNodesFromBlock B2) /\
   getTerminatorFromBlock B1 = getTerminatorFromBlock B2.
 Proof.
-  intros.
+  intros B1 B2 H.
   destruct B1.
   destruct B2. simpl in *.
   unfold tv_block in H.
   destruct (cmds2sbs c).
   destruct (cmds2sbs c0).
-  decompose [and] H. split; auto.
+  bdestruct5 H as J1 J2 J3 J4 J5.
+  sumbool_subst.
+  split; auto.
 Qed.
  
 Lemma tv_getIncomingValuesForBlockFromPHINodes : forall ps1 B1 ps2 B2,
@@ -763,14 +823,15 @@ Lemma tv_getIncomingValuesForBlockFromPHINodes : forall ps1 B1 ps2 B2,
   getIncomingValuesForBlockFromPHINodes ps1 B1 =
   getIncomingValuesForBlockFromPHINodes ps2 B2 .
 Proof.
-  induction ps1; intros.
+  induction ps1; intros B1 ps2 B2 H H0.
     destruct ps2; simpl in *; auto.
       inversion H0.
 
     destruct ps2; simpl in *.
       inversion H0.
 
-      destruct H0; subst.
+      bdestruct H0 as J1 H1.
+      sumbool_subst.
       apply IHps1 with (B1:=B1)(B2:=B2) in H1; auto.
       rewrite H1.
       apply tv_block__inv in H.
@@ -854,32 +915,38 @@ Proof.
     destruct Ps2; inversion H.
       inversion H0.
 
-    destruct a; simpl in H.
+    (product_cases (destruct a) Case); simpl in H.
+    Case "product_gvar".
       destruct Ps2; try solve [inversion H].
       simpl in H0.
-      destruct p; inversion H; subst.
+      destruct p; try solve [inversion H].
+      bdestruct H as H1 H2.
       apply IHPs1 with (fid:=fid)(rt:=rt)(la:=la)(lb1:=lb1) in H2; auto.
  
+    Case "product_fdec".
       destruct Ps2; try solve [inversion H].
       simpl in H0.
-      destruct p; inversion H; subst.
+      destruct p; try solve [inversion H].
+      bdestruct H as H1 H2.
       apply IHPs1 with (fid:=fid)(rt:=rt)(la:=la)(lb1:=lb1) in H2; auto.
 
+    Case "product_fdef".
       destruct Ps2; try solve [inversion H].
       simpl in *.
-      destruct p; inversion H; subst. 
+      destruct p; try solve [inversion H].
+      bdestruct H as H1 H2.    
       simpl in *.
       destruct f.
       destruct f0.
       unfold tv_fdef in H1.
-      destruct H1 as [EQ H1]; subst.
+      bdestruct H1 as EQ H1.
+      sumbool_subst.
       simpl in *.
       remember (getFheaderID f0) as R.
       destruct (R==fid); subst.
         inversion H0. subst b. 
         exists b0. split; auto.
 
-        destruct H.
         apply IHPs1 with (Ps2:=Ps2) in H0; auto.
 Qed.
 
@@ -1033,8 +1100,10 @@ Proof.
   unfold tv_dbCall__is__correct_prop, 
          tv_subblock__is__correct_prop, tv_subblocks__is__correct_prop,
          tv_block__is__correct_prop, tv_blocks__is__correct_prop,
-         tv_fdef__is__correct_prop; intros; subst.
+         tv_fdef__is__correct_prop.
 Case "dbCall_intro".
+  intros S TD Ps lc gl rid noret0 tailc0 rt fid lp Rid oResult tr lc' Mem0 Mem' 
+         als' Mem'' B' d H e S2 Ps2 H0 H1 H2 H3 H4 H5 H6.
   inversion d; subst.
     apply H with (S2:=S2)(Ps2:=Ps2) in H7; auto.
     clear H.
@@ -1049,6 +1118,8 @@ Case "dbCall_intro".
     split; eauto using eqAL_callUpdateLocals, eqAL_refl.
 
 Case "dbSubblock_intro".
+  intros S TD Ps lc1 als1 gl Mem1 cs call0 lc2 als2 Mem2 tr1 lc3 Mem3 tr2 d d0 H S2 
+         Ps2 cs2 sb1 sb2 H0 H1 H2 H3 H4 H5 H6 H7 H8 H9 H10.
   unfold tv_subblock in H10.
   destruct sb1.
   destruct sb2.
@@ -1060,11 +1131,13 @@ Case "dbSubblock_intro".
   apply cmds2sb_inv in H2.
   destruct H2 as [cs2' [call0 [J1 [J2 J3]]]]; subst.
   apply cmds2nbs__nbranchs2cmds in J2.
-  destruct H10 as [EQ1 EQ2]; subst.
+  bdestruct H10 as EQ1 EQ2.
+  sumbool_subst.
   inversion H7; subst.
   assert (uniq lc2) as J.
     apply se_dbCmds_preservation in d; auto.
-  apply tv_cmds__is__correct with (nbs':=NBs1) in d; eauto.
+  apply tv_cmds__is__correct with (nbs':=NBs1) in d; 
+    try solve [eauto using eq_sumbool2bool_true | apply eq_sumbool2bool_true; auto].
   destruct d as [lc2' [Hcmds Heq2]].
   apply H in H6; auto. clear H.
   destruct H6 as [lc3' [HdbCall Heq3]].  
@@ -1073,12 +1146,15 @@ Case "dbSubblock_intro".
   exists lc3''. split; eauto using eqAL_trans, eqAL_sym.
 
 Case "dbSubblocks_nil".
+  intros S TD Ps lc als gl Mem0 S2 Ps2 sbs1 sbs2 cs2 H H0 H1 H2 H3 H4 H5 H6 H7 H8 H9.
   simpl in H0. inversion H0; subst.
   destruct sbs2;try solve [auto | simpl in H9; inversion H9].
     apply cmds2sbs_nil_inv in H1; subst.
     exists lc. split; auto using eqAL_refl.
 
 Case "dbSubblocks_cons".
+  intros S TD Ps lc1 als1 gl Mem1 lc2 als2 Mem2 lc3 als3 Mem3 cs cs' t1 t2 d H d0 H0 S2
+         Ps2 sbs1 sbs2 cs2 H1 H2 H3 H4 H5 H6 H7 H8 H9 H10 H11.
   assert (Hcs2sb := d).
   apply dbSubblock__cmds2sb in Hcs2sb.
   destruct Hcs2sb as [sb Hcs2sb].
@@ -1088,11 +1164,11 @@ Case "dbSubblocks_cons".
   apply cmds_cons2sbs_inv with (sb:=sb)(sbs':=sbs) in H2; auto.
   subst.
   simpl in H11.
-  destruct sbs2 ; simpl in H11; inversion H11.
-  clear H11.
+  destruct sbs2 ; try solve [inversion H11].
+  bdestruct H11 as H2 H12.
   apply cmds2sbs_cons_inv in H3.
   destruct H3 as [cs21 [cs22 [cs212s [cs222sbs2 EQ]]]]; subst.
-  inversion H8; subst. clear H8.  
+  inversion_clear H8; subst.
   apply H with (S2:=S2)(Ps2:=Ps2)(cs2:=cs21) in H2; auto.
   clear H. destruct H2 as [lc2' [HdbSubblock Heq2]].
   assert (uniq lc2) as Uniqc2.
@@ -1104,6 +1180,8 @@ Case "dbSubblocks_cons".
   exists lc3''. split; eauto using eqAL_trans, eqAL_sym.
 
 Case "dbBlock_intro".
+  intros S TD Ps F tr1 tr2 l0 ps cs cs' tmn gl lc1 als1 Mem1 lc2 als2 Mem2 lc3 als3 Mem3 lc4 B' arg0 tr3 d H d0 d1
+         S2 Ps2 fh1 lb1 fh2 lb2 B1 lc als Mem0 B1' lc' als' Mem' B2 H0 H1 H2 H3 H4 H5 H6 H7 H8 H9 H10 H11 H12; subst.
   inversion H0; subst. clear H0.
   inversion H1; subst. clear H1.
   destruct B2 as [l2 ps2 cs2 tmn2].
@@ -1112,7 +1190,8 @@ Case "dbBlock_intro".
   remember (cmds2sbs cs2) as R2.
   destruct R1 as [sbs1 nbs1].
   destruct R2 as [sbs2 nbs2].
-  destruct H12 as [EQ1 [Htv_phinodes [Htv_subblocks [Htv_cmds EQ2]]]]; subst.
+  bdestruct5 H12 as EQ1 Htv_phinodes Htv_subblocks Htv_cmds EQ2.
+  sumbool_subst.
 
   assert (Hcs2sbs1 := d).
   apply dbSubblocks__cmds2sbs in Hcs2sbs1.
@@ -1170,9 +1249,11 @@ Case "dbBlock_intro".
     unfold tv_block.
     rewrite <- HeqR1.
     rewrite <- HeqR2.
-    split; auto.
+    repeat_bsplit.
 
 Case "dbBlocks_nil".
+  intros S TD Ps gl F arg0 state S2 Ps2 fh1 lb1 fh2 lb2 lc n tmn1 l1 ps1 cs1
+         ps1' l1' als lc' Mem0 Mem' als' tmn1' cs1' H H0 H1 H2 H3 H4 H5 H6 H7 H8 H9 H10 H11; subst.
   inversion H0; subst. clear H0.
   apply uniqSystem__uniqFdef in H4; auto.
   apply uniqSystem__uniqFdef in H5; auto.
@@ -1184,6 +1265,8 @@ Case "dbBlocks_nil".
   repeat (split; auto).
 
 Case "dbBlocks_cons".
+  intros S TD Ps gl F arg0 S1 S2 S3 t1 t2 d H d0 H0 S0 Ps2 fh1 lb1 fh2 lb2 lc n tmn1 l1
+         ps1 cs1 ps1' l1' als lc' Mem0 Mem' als' tmn1' cs1' H1 H2 H3 H4 H5 H6 H7 H8 H9 H10 H11 H12 H13; subst.
   inversion d; subst.
   assert (J:=H12).  
   assert (uniqF1:=H6).
@@ -1223,10 +1306,12 @@ Case "dbBlocks_cons".
     inversion J3; subst. clear J3.
     split; eauto using eqAL_sym, eqAL_trans.
 
-
     apply uniqFdef__wf_block with (fh:=fh2)(lb:=lb2)(n:=n); eauto using uniqSystem__uniqFdef.
 
 Case "dbFdef_func".
+    intros S TD Ps gl fid lp lc rid l1 ps1 cs1 tmn1 rt la lb Result lc1 tr1 Mem0 Mem1 als1
+           l2 ps2 cs21 cs22 lc2 als2 Mem2 tr2 lc3 als3 Mem3 tr3 e e0 d H d0 H0 d1
+           Ps2 S2 la0 lb1 H1 H2 H3 H4 H5 H6 H7 H8.
     rewrite H1 in e. inversion e; subst. clear e.
     assert (exists lb2, lookupFdefViaIDFromProducts Ps2 fid = Some (fdef_intro (fheader_intro rt fid la) lb2) /\
                         tv_blocks lb lb2) as J.
@@ -1250,7 +1335,8 @@ Case "dbFdef_func".
       remember (cmds2sbs cs2') as R2.
       destruct R1 as [sbs1 nbs1].
       destruct R2 as [sbs2 nbs2].
-      destruct J5 as [EQ1 [Htv_phinodes [Htv_subblocks [Htv_cmds EQ2]]]]; subst.
+      bdestruct5 J5 as EQ1 Htv_phinodes Htv_subblocks Htv_cmds EQ2.
+      sumbool_subst.
 
       assert (Hcs21sbs1 := d0).
       apply dbSubblocks__cmds2sbs in Hcs21sbs1.
@@ -1323,9 +1409,12 @@ Case "dbFdef_func".
       eapply lookupFdefViaIDFromProductsInSystem; eauto.
 
       unfold tv_fdef.
-      split; auto.
+      repeat_bsplit.
 
 Case "dbFdef_proc".
+    intros S TD Ps gl fid lp lc rid l1 ps1 cs1 tmn1 rt la lb lc1 tr1 Mem0 Mem1 als1
+           l2 ps2 cs21 cs22 lc2 als2 Mem2 tr2 lc3 als3 Mem3 tr3 e e0 d H d0 H0 d1
+           Ps2 S2 la0 lb1 H1 H2 H3 H4 H5 H6 H7 H8.
     rewrite H1 in e. inversion e; subst. clear e.
     assert (exists lb2, lookupFdefViaIDFromProducts Ps2 fid = Some (fdef_intro (fheader_intro rt fid la) lb2) /\
                         tv_blocks lb lb2) as J.
@@ -1349,7 +1438,8 @@ Case "dbFdef_proc".
       remember (cmds2sbs cs2') as R2.
       destruct R1 as [sbs1 nbs1].
       destruct R2 as [sbs2 nbs2].
-      destruct J5 as [EQ1 [Htv_phinodes [Htv_subblocks [Htv_cmds EQ2]]]]; subst.
+      bdestruct5 J5 as EQ1 Htv_phinodes Htv_subblocks Htv_cmds EQ2.
+      sumbool_subst.
 
       assert (Hcs21sbs1 := d0).
       apply dbSubblocks__cmds2sbs in Hcs21sbs1.
@@ -1421,7 +1511,7 @@ Case "dbFdef_proc".
       eapply lookupFdefViaIDFromProductsInSystem; eauto.
 
       unfold tv_fdef.
-      split; auto.
+      repeat_bsplit.
 Qed.   
 
 Lemma tv_dbCall__is__correct : forall S1 TD Ps1 gl lc Mem0 call0 lc' Mem' tr S2 Ps2,
